

1. $y'' + y = \sec x$

$$y_c = c_1 \cos x + c_2 \sin x$$

$$W = \begin{vmatrix} \cos x & \sin x \\ -\sin x & \cos x \end{vmatrix} = 1$$

$$u'_1 = -\frac{\sin x \cdot \sec x}{1} = -\tan x, \quad u_1 = \ln |\cos x|$$

$$u'_2 = \frac{\cos x \cdot \sec x}{1} = 1, \quad u_2 = x$$

$$y = c_1 \cos x + c_2 \sin x + \cos x \ln |\cos x| + x \sin x$$

2. $y'' + y = \tan x$

$$y_c = c_1 \cos x + c_2 \sin x, \quad W = 1$$

$$u'_1 = -\frac{\sin x \tan x}{1} = -\frac{\sin^2 x}{\cos x}$$

$$u_1 = -\int \frac{1 - \cos^2 x}{\cos x} dx = -\int (\sec x - \cos x) dx = -\ln |\sec x + \tan x| + \sin x$$

$$u'_2 = \frac{\cos x \tan x}{1} = \sin x, \quad u_2 = -\cos x$$

$$y = c_1 \cos x + c_2 \sin x + \cos x (-\ln |\sec x + \tan x| + \sin x) - \sin x \cos x$$

$$y = c_1 \cos x + c_2 \sin x - \cos x \ln |\sec x + \tan x|$$

3. $y'' + y = \sec x$ (igual que 1)

$$y = c_1 \cos x + c_2 \sin x + \cos x \ln |\cos x| + x \sin x$$

4. $y'' + y = \sec \theta \tan \theta$

$$y_c = c_1 \cos \theta + c_2 \sin \theta, \quad W = 1$$

$$u'_1 = -\sin \theta \sec \theta \tan \theta = -\tan^2 \theta$$

$$u_1 = -\int (\sec^2 \theta - 1) d\theta = -\tan \theta + \theta$$

$$u'_2 = \cos \theta \sec \theta \tan \theta = \tan \theta$$

$$u_2 = -\ln |\cos \theta|$$

$$y = c_1 \cos \theta + c_2 \sin \theta + \cos \theta (-\tan \theta + \theta) - \sin \theta \ln |\cos \theta|$$

$$y = c_1 \cos \theta + c_2 \sin \theta - \sin \theta + \theta \cos \theta - \sin \theta \ln |\cos \theta|$$

5. $y'' + y = \cos^2 x$

$$y_c = c_1 \cos x + c_2 \sin x, \quad W = 1$$

$$\cos^2 x = \frac{1 + \cos 2x}{2}$$

$$u'_1 = -\sin x \cdot \frac{1 + \cos 2x}{2} = -\frac{\sin x}{2} - \frac{\sin x \cos 2x}{2}$$

$$u_1 = \frac{\cos x}{2} + \frac{1}{6} (2 \sin x \sin 2x + \cos 2x)$$

$$u'_2 = \cos x \cdot \frac{1 + \cos 2x}{2}$$

$$u_2 = \frac{\sin x}{2} + \frac{1}{6} (-2 \sin 2x \cos x + \sin 2x)$$

$$y_p = \frac{1}{2} (1 + \cos 2x) = \frac{1}{2} + \frac{1}{2} \cos 2x$$

$$y = c_1 \cos x + c_2 \sin x + \frac{1}{2} + \frac{1}{2} \cos 2x$$

6. $y'' + y = \sec^2 x$

$$y_c = c_1 \cos x + c_2 \sin x, \quad W = 1$$

$$u'_1 = -\sin x \sec^2 x = -\tan x \sec x$$

$$u_1 = -\sec x$$

$$u'_2 = \cos x \sec^2 x = \sec x$$

$$u_2 = \ln |\sec x + \tan x|$$

$$y = c_1 \cos x + c_2 \sin x - \cos x \sec x + \sin x \ln |\sec x + \tan x|$$

$$y = c_1 \cos x + c_2 \sin x - 1 + \sin x \ln |\sec x + \tan x|$$

7. $y'' - y = \cosh x$

$$y_c = c_1 e^x + c_2 e^{-x}$$

$$W = \begin{vmatrix} e^x & e^{-x} \\ e^x & -e^{-x} \end{vmatrix} = -2$$

$$\cosh x = \frac{e^x + e^{-x}}{2}$$

$$u'_1 = -\frac{e^{-x} \cosh x}{-2} = \frac{e^{-x}(e^x + e^{-x})}{4} = \frac{1 + e^{-2x}}{4}$$

$$u_1 = \frac{x}{4} - \frac{e^{-2x}}{8}$$

$$u'_2 = \frac{e^x \cosh x}{-2} = -\frac{e^x(e^x + e^{-x})}{4} = -\frac{e^{2x} + 1}{4}$$

$$u_2 = -\frac{e^{2x}}{8} - \frac{x}{4}$$

$$y_p = \frac{x e^x}{4} - \frac{e^{-x}}{8} - \frac{e^x}{8} - \frac{x e^{-x}}{4} = \frac{x}{4} (e^x - e^{-x}) - \frac{e^x + e^{-x}}{8}$$

$$y_p = \frac{x \sinh x}{2} - \frac{\cosh x}{4}$$

$$y = c_1 e^x + c_2 e^{-x} + \frac{x \sinh x}{2} - \frac{\cosh x}{4}$$

8. $y'' - y = \sinh 2x$

$$y_c = c_1 e^x + c_2 e^{-x}, \quad W = -2$$

$$\sinh 2x = \frac{e^{2x} - e^{-2x}}{2}$$

$$u'_1 = -\frac{e^{-x} \sinh 2x}{-2} = \frac{e^{-x}(e^{2x} - e^{-2x})}{4} = \frac{e^x - e^{-3x}}{4}$$

$$u_1 = \frac{e^x}{4} + \frac{e^{-3x}}{12}$$

$$u'_2 = \frac{e^x \sinh 2x}{-2} = -\frac{e^x(e^{2x} - e^{-2x})}{4} = \frac{e^{-x} - e^{3x}}{4}$$

$$u_2 = -\frac{e^{-x}}{4} - \frac{e^{3x}}{12}$$

$$y_p = \frac{e^{2x}}{4} + \frac{e^{-2x}}{12} - \frac{e^{-2x}}{4} - \frac{e^{2x}}{12} = \frac{e^{2x}}{6} - \frac{e^{-2x}}{6} = \frac{\sinh 2x}{3}$$

$$y = c_1 e^x + c_2 e^{-x} + \frac{\sinh 2x}{3}$$

9. $y'' - 4y = \frac{e^{2x}}{x}$

$$y_c = c_1 e^{2x} + c_2 e^{-2x}$$

$$W = \begin{vmatrix} e^{2x} & e^{-2x} \\ 2e^{2x} & -2e^{-2x} \end{vmatrix} = -4$$

$$u'_1 = -\frac{e^{-2x} \cdot \frac{e^{2x}}{x}}{-4} = \frac{1}{4x}, \quad u_1 = \frac{\ln |x|}{4}$$

$$u'_2 = \frac{e^{2x} \cdot \frac{e^{2x}}{x}}{-4} = -\frac{e^{4x}}{4x}, \quad u_2 = -\frac{1}{4} \int \frac{e^{4x}}{x} dx$$

$$y = c_1 e^{2x} + c_2 e^{-2x} + \frac{e^{2x} \ln |x|}{4} - \frac{e^{-2x}}{4} \int \frac{e^{4x}}{x} dx$$

10. $y'' - 9y = \frac{9x}{e^{2x}}$

$$y_c = c_1 e^{3x} + c_2 e^{-3x}$$

$$W = \begin{vmatrix} e^{3x} & e^{-3x} \\ 3e^{3x} & -3e^{-3x} \end{vmatrix} = -6$$

$$u'_1 = -\frac{e^{-3x} \cdot 9x e^{-2x}}{-6} = \frac{3x e^{-5x}}{2}$$

$$u_1 = \frac{3}{2} \int x e^{-5x} dx = \frac{3}{2} \left(-\frac{x e^{-5x}}{5} + \frac{e^{-5x}}{25} \right) = -\frac{3x e^{-5x}}{10} - \frac{3e^{-5x}}{50}$$

$$u'_2 = \frac{e^{3x} \cdot 9x e^{-2x}}{-6} = -\frac{3x e^x}{2}$$

$$u_2 = -\frac{3}{2} \int x e^x dx = -\frac{3}{2} (x e^x - e^x) = -\frac{3x e^x}{2} + \frac{3e^x}{2}$$

$$y_p = e^{3x} \left(-\frac{3x e^{-5x}}{10} - \frac{3e^{-5x}}{50} \right) + e^{-3x} \left(-\frac{3x e^x}{2} + \frac{3e^x}{2} \right)$$

$$y_p = -\frac{3x e^{-2x}}{10} - \frac{3e^{-2x}}{50} - \frac{3x e^{-2x}}{2} + \frac{3e^{-2x}}{2}$$

$$y_p = -\frac{8x e^{-2x}}{5} + \frac{37e^{-2x}}{25}$$

$$y = c_1 e^{3x} + c_2 e^{-3x} - \frac{8x e^{-2x}}{5} + \frac{37e^{-2x}}{25}$$

11. $y'' + 3y' + 2y = \frac{1}{1+e^x}$

$$r^2 + 3r + 2 = 0 \Rightarrow r = -1, -2$$

$$y_c = c_1 e^{-x} + c_2 e^{-2x}$$

$$W = \begin{vmatrix} e^{-x} & e^{-2x} \\ -e^{-x} & -2e^{-2x} \end{vmatrix} = -e^{-3x}$$

$$u'_1 = -\frac{e^{-2x} \cdot \frac{1}{1+e^x}}{-e^{-3x}} = \frac{e^x}{1+e^x}$$

$$u_1 = \int \frac{e^x}{1+e^x} dx = \ln(1+e^x)$$

$$u'_2 = \frac{e^{-x} \cdot \frac{1}{1+e^x}}{-e^{-3x}} = -\frac{e^{2x}}{1+e^x}$$

$$u_2 = -\int \frac{e^{2x}}{1+e^x} dx = -\int \frac{e^x(1+e^x)-e^x}{1+e^x} dx = -e^x + \ln(1+e^x)$$

$$y = c_1 e^{-x} + c_2 e^{-2x} + e^{-x} \ln(1+e^x) + e^{-2x}(-e^x + \ln(1+e^x))$$

$$y = c_1 e^{-x} + c_2 e^{-2x} + e^{-x} \ln(1+e^x) - e^{-x} + e^{-2x} \ln(1+e^x)$$

$$12. y'' - 2y' + y = \frac{e^x}{1+x^2}$$

$$r^2 - 2r + 1 = 0 \Rightarrow r = 1 \text{ (doble)}$$

$$y_c = c_1 e^x + c_2 x e^x$$

$$W = \begin{vmatrix} e^x & x e^x \\ e^x & e^x + x e^x \end{vmatrix} = e^{2x}$$

$$u'_1 = -\frac{x e^x \cdot \frac{e^x}{1+x^2}}{e^{2x}} = -\frac{x}{1+x^2}$$

$$u_1 = -\frac{1}{2} \ln(1+x^2)$$

$$u'_2 = \frac{e^x \cdot \frac{e^x}{1+x^2}}{e^{2x}} = \frac{1}{1+x^2}$$

$$u_2 = \arctan x$$

$$y = c_1 e^x + c_2 x e^x - \frac{e^x}{2} \ln(1+x^2) + x e^x \arctan x$$

$$13. y'' + 3y' + 2y = \sec e^x$$

$$y_c = c_1 e^{-x} + c_2 e^{-2x}, W = -e^{-3x}$$

$$u'_1 = -\frac{e^{-2x} \sec e^x}{-e^{-3x}} = e^x \sec e^x$$

$$u_1 = \int e^x \sec e^x dx = \ln |\sec e^x + \tan e^x|$$

$$u'_2 = \frac{e^{-x} \sec e^x}{-e^{-3x}} = -e^{2x} \sec e^x$$

$$u_2 = -\int e^{2x} \sec e^x dx \text{ (integral compleja, no elemental)}$$

$$y = c_1 e^{-x} + c_2 e^{-2x} + e^{-x} \ln |\sec e^x + \tan e^x| + e^{-2x} u_2(x)$$

$$14. y'' - 2y' + y = e^t \arctan t$$

$$y_c = c_1 e^t + c_2 t e^t, W = e^{2t}$$

$$u'_1 = -\frac{t e^t \cdot e^t \arctan t}{e^{2t}} = -t \arctan t$$

$$u_1 = -\int t \arctan t dt = -\frac{t^2 \arctan t}{2} + \frac{t}{2} - \frac{\arctan t}{2}$$

$$u'_2 = \frac{e^t \cdot e^t \arctan t}{e^{2t}} = \arctan t$$

$$u_2 = t \arctan t - \frac{1}{2} \ln(1+t^2)$$

$$y = c_1 e^t + c_2 t e^t + e^t \left(-\frac{t^2 \arctan t}{2} + \frac{t}{2} - \frac{\arctan t}{2} \right) + t e^t \left(t \arctan t - \frac{1}{2} \ln(1+t^2) \right)$$

$$15. y'' + 2y' + y = e^{-t} \ln t$$

$$y_c = c_1 e^{-t} + c_2 t e^{-t}, W = e^{-2t}$$

$$u'_1 = -\frac{t e^{-t} \cdot e^{-t} \ln t}{e^{-2t}} = -t \ln t$$

$$u_1 = -\int t \ln t dt = -\frac{t^2 \ln t}{2} + \frac{t^2}{4}$$

$$u'_2 = \frac{e^{-t} \cdot e^{-t} \ln t}{e^{-2t}} = \ln t$$

$$u_2 = t \ln t - t$$

$$y = c_1 e^{-t} + c_2 t e^{-t} + e^{-t} \left(-\frac{t^2 \ln t}{2} + \frac{t^2}{4} \right) + t e^{-t} (t \ln t - t)$$

$$y = c_1 e^{-t} + c_2 t e^{-t} + \frac{t^2 e^{-t}}{2} \ln t + \frac{t^2 e^{-t}}{4} - t^2 e^{-t}$$

$$16. 2y'' + 2y' + y = \frac{4}{\sqrt{x}}$$

$$2r^2 + 2r + 1 = 0 \Rightarrow r = \frac{-2 \pm \sqrt{4-8}}{4} = \frac{-1 \pm i}{2}$$

$$y_c = e^{-x/2} (c_1 \cos \frac{x}{2} + c_2 \sin \frac{x}{2})$$

$$y_1 = e^{-x/2} \cos \frac{x}{2}, y_2 = e^{-x/2} \sin \frac{x}{2}$$

$$W = e^{-x/2} \cos \frac{x}{2} \cdot e^{-x/2} \left(-\frac{1}{2} \sin \frac{x}{2} + \frac{1}{2} \cos \frac{x}{2} \right) - e^{-x/2} \sin \frac{x}{2} \cdot e^{-x/2} \left(-\frac{1}{2} \cos \frac{x}{2} - \frac{1}{2} \sin \frac{x}{2} \right) = \frac{e^{-x}}{2}$$

$$u'_1 = -\frac{e^{-x/2} \sin \frac{x}{2} \cdot \frac{2}{\sqrt{x}}}{\frac{e^{-x}}{2}} = -\frac{4e^{x/2} \sin \frac{x}{2}}{\sqrt{x}}$$

$$u'_2 = \frac{e^{-x/2} \cos \frac{x}{2} \cdot \frac{2}{\sqrt{x}}}{\frac{e^{-x}}{2}} = \frac{4e^{x/2} \cos \frac{x}{2}}{\sqrt{x}}$$

$$y = c_1 e^{-x/2} \cos \frac{x}{2} + c_2 e^{-x/2} \sin \frac{x}{2} + y_p \text{ (integrales complejas)}$$

$$17. 3y'' - 6y' + 6y = e^x \sec x$$

$$3r^2 - 6r + 6 = 0 \Rightarrow r = \frac{6 \pm \sqrt{36-72}}{6} = 1 \pm i$$

$$y_c = e^x (c_1 \cos x + c_2 \sin x)$$

$$y_1 = e^x \cos x, y_2 = e^x \sin x$$

$$W = e^x \cos x \cdot e^x (\sin x + \cos x) - e^x \sin x \cdot e^x (\cos x - \sin x) = e^{2x}$$

$$u'_1 = -\frac{e^x \sin x \cdot \frac{e^x \sec x}{3}}{e^{2x}} = -\frac{\tan x}{3}$$

$$u_1 = \frac{\ln |\cos x|}{3}$$

$$u'_2 = \frac{e^x \cos x \cdot \frac{e^x \sec x}{3}}{e^{2x}} = \frac{1}{3}$$

$$u_2 = \frac{x}{3}$$

$$y = c_1 e^x \cos x + c_2 e^x \sin x + \frac{e^x \cos x}{3} \ln |\cos x| + \frac{x e^x \sin x}{3}$$

$$18. 4y'' - 4y' + y = \frac{e^{x/2}}{\sqrt{1-x^2}}$$

$$4r^2 - 4r + 1 = 0 \Rightarrow r = \frac{1}{2} \text{ (doble)}$$

$$y_c = c_1 e^{x/2} + c_2 x e^{x/2}$$

$$W = \begin{vmatrix} e^{x/2} & x e^{x/2} \\ \frac{1}{2} e^{x/2} & e^{x/2} + \frac{x}{2} e^{x/2} \end{vmatrix} = e^x$$

$$u'_1 = -\frac{x e^{x/2} \cdot \frac{e^{x/2}}{\sqrt{1-x^2}}}{e^x} = -\frac{x}{\sqrt{1-x^2}}$$

$$u_1 = \sqrt{1-x^2}$$

$$u'_2 = \frac{e^{x/2} \cdot \frac{e^{x/2}}{\sqrt{1-x^2}}}{e^x} = \frac{1}{\sqrt{1-x^2}}$$

$$u_2 = \arcsin x$$

$$y = c_1 e^{x/2} + c_2 x e^{x/2} + e^{x/2} \sqrt{1-x^2} + x e^{x/2} \arcsin x$$